Language.v
@@ -2,6 +2,9 @@ Require Import Arith List Alphabet.
 
 Section Language.
   Local Lemma two_gte_one: 2 >= 1. Proof. auto. Qed.
-  Definition binstr := str (nat_to_atl 1 2 two_gte_one).
-  Definition language := binstr -> Prop.
+  Definition bitstr := str (nat_to_atl 1 2 two_gte_one).
+  Definition language := bitstr -> Prop.
+
+  Axiom lang_extensionality: forall (l m: language),
+    l = m <-> forall (w: bitstr), l w <-> m w.
 End Language.
