Turing.v
@@ -79,3 +79,172 @@ Section Turing.
       m s (head r) s' sym' d = true ->
       step m (s, l, r) (go_d d (s', l, r) sym').
 End Turing.
+
+Section RunTuring.
+  Context {state_count symbol_count: positive}.
+
+  Local Definition machine := turing_machine state_count symbol_count.
+  Local Definition state := alphabet state_count.
+  Local Definition symbol := alphabet symbol_count.
+  Local Definition tape := str symbol_count.
+  Local Definition State: Set := state * tape * tape.
+  Local Definition blank := sym_0 symbol_count.
+  Local Definition initial := sym_0 state_count.
+
+  Variable m: machine.
+  Variable program input: tape.
+  Local Definition Initial: State := (initial, program, input).
+  Local Definition m_step := step m.
+  Local Definition m_steps := steps m_step.
+
+  Local Definition tm_halts := halts Initial m_step.
+  Local Definition tm_halted (s: State) := halted s m_step.
+
+  Local Definition m_runtime_func := runtime_func Initial m_step.
+
+  Local Definition next_steps_point (s: State) (i: state) (j: symbol): list State :=
+    let (st'l, r) := s in let (st, l) := st'l in
+    match m st (head r) i j Left with
+    | false => nil
+    | true => cons (go_left (i, l, r) j) nil
+    end ++
+    match m st (head r) i j Right with
+    | false => nil
+    | true => cons (go_right (i, l, r) j) nil
+    end.
+
+  Local Lemma next_steps_point_correct:
+    forall (s s': State),
+    let (st'l, r) := s' in let (st, l) := st'l in
+    m_step s s' -> In s' (next_steps_point s st (head (tail r))) \/
+                   In s' (next_steps_point s st (head l)).
+  Proof.
+    destruct s as [st'l r].
+    destruct st'l as [st l].
+    destruct s' as [st'l' r'].
+    destruct st'l' as [st' l'].
+    intros.
+    unfold next_steps_point.
+    inversion H; subst.
+    assert (head (head r :: sym' :: tail r) = head r). unfold head. unfold hd. auto.
+    destruct d.
+    - left.
+      unfold go_d in H5.
+      remember H5 as H7. clear HeqH7.
+      apply go_left_state in H7.
+      apply go_left_sym in H5.
+      rewrite <- H5.
+      rewrite <- H7.
+      rewrite H2. simpl. auto.
+    - right.
+      unfold go_d in H5.
+      remember H5 as H7. clear HeqH7.
+      apply go_right_state in H7.
+      apply go_right_sym in H5.
+      rewrite <- H5.
+      rewrite <- H7.
+      rewrite H2. simpl.
+      intuition.
+  Qed.
+
+  Local Lemma next_steps_point_correct':
+    forall (s s': State), m_step s s' ->
+    exists (st: state) (sym: symbol), In s' (next_steps_point s st sym).
+  Proof.
+    intros.
+    remember (next_steps_point_correct s s').
+    destruct s'.
+    destruct p.
+    apply y in H.
+    destruct H; eauto.
+  Qed.
+
+  Definition next_steps (s: State): list State :=
+    flat_map
+      (fun sym =>
+         flat_map (fun st => next_steps_point s st sym) (all_syms state_count)
+      )
+      (all_syms symbol_count).
+
+  Theorem next_steps_correct: forall (s s': State), m_step s s' <-> In s' (next_steps s).
+  Proof.
+    split; intros.
+    - apply next_steps_point_correct' in H.
+      destruct H.
+      destruct H.
+      unfold next_steps.
+      apply in_flat_map.
+      exists x0.
+      split.
+      apply all_syms_correct.
+      apply in_flat_map.
+      exists x.
+      split.
+      apply all_syms_correct.
+      exact H.
+    - unfold next_steps in H.
+      apply in_flat_map in H.
+      destruct H.
+      destruct H.
+      clear H.
+      apply in_flat_map in H0.
+      destruct H0.
+      destruct H.
+      clear H.
+  Admitted.
+
+  Definition is_halted (s: State) :=
+    match next_steps s with
+    | nil => true
+    | _ => false
+    end.
+
+  Theorem is_halted_correct: forall (s: State), tm_halted s <-> is_halted s = true.
+  Proof.
+    intros.
+    unfold is_halted.
+    unfold tm_halted.
+    unfold halted.
+    split; intros.
+    - destruct (next_steps s) eqn:Hs; auto.
+      remember (List.in_eq s0 l) as Hin.
+      clear HeqHin.
+      rewrite <- Hs in Hin.
+      apply <- next_steps_correct in Hin.
+      exfalso.
+      exact (H s0 Hin).
+    - intro.
+      destruct (next_steps s) eqn:Hs.
+      + apply next_steps_correct in H0.
+        rewrite Hs in H0.
+        exact (List.in_nil H0).
+      + inversion H.
+  Qed.
+
+  Definition read_decision (s: State) :=
+    let (st'l, r) := s in
+    match sym_to_nat (head r) with
+    | 0 => false
+    | _ => true
+    end.
+
+  Inductive decision': State -> bool -> Prop :=
+  | Rejects: tm_halts -> forall (init: State), (
+      forall (l r: tape) (s: state),
+        tm_halted (s, l, r) -> m_steps init (s, l, r) -> sym_to_nat (head r) = 0
+    ) -> decision' init false
+  | Accepts: tm_halts -> forall (init: State), (
+      exists (l r: tape) (s: state),
+        tm_halted (s, l, r) /\ m_steps init (s, l, r) /\ sym_to_nat (head r) <> 0
+    ) -> decision' init true.
+
+  Fixpoint simulate (n: nat) (s: State): option bool :=
+    if is_halted s then Some (read_decision s)
+    else None.
+
+  Theorem simulate_correct:
+    forall (b: bool) (s: State), decision' s b <-> exists (n: nat), simulate n s = Some b.
+  Proof.
+
+  Qed.
+End RunTuring.
