Computation.v
@@ -1,0 +1,175 @@
+Require Import List Relations Arith Alphabet Bool Language.
+
+Section Computation.
+  Context {state: Type}.
+  Variable step_rel: relation state.
+  Variable accepting_state: state -> Prop.
+  Variable encode_input: bitstr -> state.
+
+  Definition deterministic :=
+    forall (s s' s'': state), step_rel s s' -> step_rel s s'' -> s' = s''.
+
+  Definition decision_model: Type := (relation state) * (state -> Prop) * (bitstr -> state).
+  Local Definition dm := (step_rel, accepting_state, encode_input).
+  Definition dm_class := decision_model -> Prop.
+
+  Inductive steps: relation state :=
+  | stepsRefl: forall (s: state), steps s s
+  | stepsOnce: forall (s s' s'': state),
+      steps s s' /\ step_rel s' s'' -> steps s s''.
+
+  Definition halted (s: state) := forall (s': state), ~step_rel s s'.
+
+  Definition runtime_f (initial: state) (f: state -> nat) :=
+    forall (s s': state), steps initial s -> step_rel s s' -> f s > f s'.
+
+  Definition halts (initial: state) :=
+    exists (f: state -> nat), runtime_f initial f.
+
+  Definition halts_within (initial: state) (n: nat) :=
+    exists (f: state -> nat), runtime_f initial f /\ f initial = n.
+
+  Lemma halts_halts_within:
+    forall (initial: state), halts initial -> exists (n: nat), halts_within initial n.
+  Proof.
+    intros.
+    destruct H as [f].
+    exists (f initial).
+    unfold halts_within.
+    exists f.
+    auto.
+  Qed.
+
+  Lemma halts_within_monotone:
+    forall (initial: state) (n m: nat), n < m ->
+    halts_within initial n -> halts_within initial m.
+  Proof.
+    intros.
+    destruct H0 as [f].
+    destruct H0.
+    unfold halts_within.
+    apply Nat.le_exists_sub in H.
+    destruct H.
+    destruct H.
+    exists (fun s => x + S (f s)).
+    unfold runtime_f.
+    rewrite H1.
+    intuition.
+  Qed.
+
+  Definition runtime (initial: state) (t: nat) :=
+    halts_within initial t /\ forall t', t' < t -> ~halts_within initial t'.
+
+  Lemma runtime_unique:
+    forall (initial: state) (t t': nat),
+    runtime initial t -> runtime initial t' -> t = t'.
+  Proof.
+    intros.
+    destruct (t ?= t') eqn: Hc.
+    - apply Nat.compare_eq_iff in Hc. auto.
+    - exfalso.
+      apply Nat.compare_lt_iff in Hc.
+      unfold runtime in H, H0.
+      destruct H, H0.
+      exact (H2 t Hc H).
+    - exfalso.
+      apply Nat.compare_gt_iff in Hc.
+      unfold runtime in H, H0.
+      destruct H, H0.
+      exact (H1 t' Hc H0).
+  Qed.
+
+  Lemma runtime_exists:
+    forall (initial: state), halts initial -> exists (t: nat), runtime initial t.
+  Proof.
+    intros.
+    apply halts_halts_within in H.
+    destruct H as [t].
+    unfold runtime.
+    induction t.
+    - exists 0.
+      intuition.
+      inversion H0.
+    - 
+  Qed.
+
+  Lemma runtime_monotone:
+
+  Definition halts' (input: bitstr) := halts (encode_input input).
+
+  Inductive decision: state -> bool -> Prop :=
+  | decisionRejects: forall (s: state),
+      halts s -> (forall (s': state), steps s s' -> halted s' -> ~accepting_state s') ->
+      decision s false
+  | decisionAccepts: forall (s: state),
+      halts s -> (exists (s': state), steps s s' /\ halted s' /\ accepting_state s') ->
+      decision s true.
+
+  Lemma not_accept_reject: forall (s: state), ~(decision s false /\ decision s true).
+  Proof.
+    intro. intro.
+    destruct H.
+    inversion H. inversion H0. subst. clear H H0.
+    destruct H5.
+    specialize H2 with x.
+    intuition.
+  Qed.
+
+  Definition decision' (w: bitstr) (b: bool) := decision (encode_input w) b.
+  Definition rejects (w: bitstr) := decision' w false.
+  Definition accepts (w: bitstr) := decision' w true.
+
+  Lemma not_accept_reject': forall (w: bitstr), ~(rejects w /\ accepts w).
+  Proof.
+    intro.
+    unfold rejects.
+    unfold decision'.
+    apply not_accept_reject.
+  Qed.
+
+  Definition next_steps_f (f: state -> list state) :=
+    forall (s s': state), step_rel s s' <-> In s' (f s).
+
+  Lemma next_steps_f_halt_dec:
+    forall f, next_steps_f f -> forall (s: state), {halted s} + {~halted s}.
+  Proof.
+    unfold next_steps_f.
+    intros.
+    unfold halted.
+    destruct (f s) eqn: Hfs.
+    - left. intros.
+      specialize H with s s'.
+      rewrite Hfs in H.
+      intuition.
+    - right.
+      intro.
+      specialize H0 with s0.
+      specialize H with s s0.
+      rewrite Hfs in H.
+      intuition.
+  Qed.
+
+  Theorem next_steps_comp_halt_decision:
+    forall f, next_steps_f f ->
+    forall (init: state), halts init -> {decision init false} + {decision init true}.
+  Proof.
+    unfold next_steps_f.
+    unfold halts.
+    intros.
+  Qed.
+
+  Definition decides (l: language): Prop :=
+    forall (w: bitstr), halts' w /\ (accepts w <-> l w).
+End Computation.
+
+Section Simulation.
+  Definition decidable {state: Type} (c: @dm_class state) (l: language) :=
+    exists (dm: decision_model), c dm /\
+    let (sr'as, encode_input) := dm in
+    let (step_rel, accepting_state) := sr'as in
+    decides step_rel accepting_state encode_input l.
+
+  Definition simulates {state: Type} (c c': @dm_class state) :=
+    forall (l: language), decidable c' l -> decidable c l.
+
+End Simulation.
