UTM.v
@@ -1,4 +1,4 @@
-Require Import Turing Run Alphabet Language.
+Require Import Turing Alphabet Language.
 
 (*
   Symbols: blank 0 1 cursor
@@ -12,10 +12,5 @@ Require Import Turing Run Alphabet Language.
  *)
 
 Section UniversalTM.
-  Print decision.
 
-  Definition tm_universal {state_count symbol_count: positive}
-    (m: machine state_count symbol_count) :=
-    forall (state_count' symbol_count': positive) (m': machine state_count' symbol_count')
-    (str: binstr) (b: bool), 
 End UniversalTM.
